add struct accessors

theories/base.v
@@ -13,3 +13,13 @@ Global Set Keyed Unification.
 Global Set Default Goal Selector "!".
 
 Arguments set _ _ _ _ _ !_ /.
+
+(* This has as better performance characteristic wrt. simpl compared
+to list_find since list_find_idx does not contain prod_map. *)
+Definition list_find_idx {A} P `{∀ x, Decision (P x)} : list A → option nat :=
+  fix go l :=
+  match l with
+  | [] => None
+  | x :: l => if decide (P x) then Some 0%nat else S <$> go l
+  end.
+Instance: Params (@list_find_idx) 3 := {}.
