theories/example.v
@@ -271,6 +271,10 @@ Qed.
   (write-reg |PSTATE| ((_ field |V|)) (_ struct (|GE| v27) (|F| #b1) (|UAO| v23) (|C| v3461) (|SP| #b1) (|N| v3459) (|Q| v21) (|A| #b1) (|SS| #b0) (|E| v33) (|TCO| v13) (|I| #b1) (|PAN| v35) (|M| v12) (|D| #b1) (|nRW| #b0) (|EL| #b00) (|IT| v31) (|IL| #b0) (|Z| v3460) (|BTYPE| v19) (|SSBS| v28) (|T| v16) (|J| v32) (|V| v3462) (|DIT| #b0))))
 *)
 Definition trc_cmp_x1_0 : trc := [
+  Smt (DeclareConst 15 (Ty_BitVec 1)) Mk_annot;
+  Smt (DeclareConst 20 (Ty_BitVec 1)) Mk_annot;
+  Smt (DeclareConst 25 (Ty_BitVec 1)) Mk_annot;
+  Smt (DeclareConst 29 (Ty_BitVec 1)) Mk_annot;
   Smt (DeclareConst 3370 (Ty_BitVec 64)) Mk_annot;
   Smt (DefineConst 3371 (Val (Val_Symbolic 3370) Mk_annot)) Mk_annot;
   ReadReg "R1" nil (Val_Symbolic 3371) Mk_annot;
@@ -493,6 +497,18 @@ Definition test_state2_local (n1 : Z) := {|
   seq_trace  := [];
   seq_regs   :=
     <[ "R1" := Val_Bits [BV{64} n1] ]> $
+    <[ "PSTATE" := (Val_Struct
+          [("GE", Val_Poison); ("F", Val_Bits [BV{1} 1]);
+          ("UAO", Val_Poison); ("C", Val_Bits [BV{1} 0]);
+          ("SP", Val_Poison); ("N", Val_Bits [BV{1} 0]);
+          ("Q", Val_Poison); ("A", Val_Bits [BV{1} 1]); ("SS", Val_Bits [BV{1} 0]);
+          ("E", Val_Poison); ("TCO", Val_Poison); ("I", Val_Bits [BV{1} 1]);
+          ("PAN", Val_Poison); ("M", Val_Poison); ("D", Val_Bits [BV{1} 1]);
+          ("nRW", Val_Bits [BV{1} 0]); ("EL", Val_Bits [BV{1} 0]);
+          ("IT", Val_Poison); ("IL", Val_Bits [BV{1} 0]);
+          ("Z", Val_Bits [BV{1} 0]); ("BTYPE", Val_Poison);
+          ("SSBS", Val_Poison); ("T", Val_Poison); ("J", Val_Poison);
+          ("V", Val_Bits [BV{1} 0]); ("DIT", Val_Bits [BV{1} 0])]) ]> $
     <[ "_PC" := Val_Bits start_address ]> $
     <[ "__PC_changed" := Val_Bool false ]> $
                                              ∅;
@@ -511,6 +527,192 @@ Definition test_state2_global  := {|
     <[0x0000000010300114 := [trc_ret]]> $
     ∅
 |}.
+
+Definition test_state2_spec : list seq_label := [ SInstrTrap 0x0000000010300018 ].
+
+Lemma ite_bits b n1 n2 :
+  ite b (Val_Bits n1) (Val_Bits n2) = Val_Bits (ite b n1 n2).
+Proof. by destruct b. Qed.
+
+Lemma test_state2_iris `{!islaG Σ} `{!threadG} n1 :
+  instr 0x0000000010300000 (Some [trc_cmp_x1_0]) -∗
+  instr 0x0000000010300004 (Some trc_bne_0xc ) -∗
+  instr 0x0000000010300008 (Some [trc_mov_x0_1]) -∗
+  instr 0x000000001030000c (Some [trc_b_0x8]) -∗
+  instr 0x0000000010300010 (Some [trc_bl_0x100]) -∗
+  instr 0x0000000010300014 (Some [trc_mov_OUT_x0]) -∗
+  instr 0x0000000010300110 (Some [trc_mov_w0_0]) -∗
+  instr 0x0000000010300114 (Some [trc_ret]) -∗
+
+  "_PC" ↦ᵣ Val_Bits start_address -∗
+  "__PC_changed" ↦ᵣ Val_Bool false -∗
+  "R30" ↦ᵣ Val_Poison -∗
+  "R1" ↦ᵣ Val_Bits [BV{64} n1] -∗
+  "R0" ↦ᵣ Val_Poison -∗
+  "OUT" ↦ᵣ Val_Poison -∗
+  "PSTATE" ↦ᵣ (Val_Struct
+          [("GE", Val_Poison); ("F", Val_Bits [BV{1} 1]);
+          ("UAO", Val_Poison); ("C", Val_Bits [BV{1} 0]);
+          ("SP", Val_Poison); ("N", Val_Bits [BV{1} 0]);
+          ("Q", Val_Poison); ("A", Val_Bits [BV{1} 1]); ("SS", Val_Bits [BV{1} 0]);
+          ("E", Val_Poison); ("TCO", Val_Poison); ("I", Val_Bits [BV{1} 1]);
+          ("PAN", Val_Poison); ("M", Val_Poison); ("D", Val_Bits [BV{1} 1]);
+          ("nRW", Val_Bits [BV{1} 0]); ("EL", Val_Bits [BV{1} 0]);
+          ("IT", Val_Poison); ("IL", Val_Bits [BV{1} 0]);
+          ("Z", Val_Bits [BV{1} 0]); ("BTYPE", Val_Poison);
+          ("SSBS", Val_Poison); ("T", Val_Poison); ("J", Val_Poison);
+          ("V", Val_Bits [BV{1} 0]); ("DIT", Val_Bits [BV{1} 0])]) -∗
+  spec_trace test_state_spec -∗
+  WPasm [].
+Proof.
+  iStartProof.
+  repeat liAStep; liShow.
+  rewrite ite_bits.
+  repeat liAStep; liShow.
+  rewrite ite_bits.
+  repeat liAStep; liShow.
+  rewrite ite_bits.
+  do 10 liAStep; liShow.
+  do 10 liAStep; liShow.
+  liAStep; liShow.
+  liAStep; liShow.
+  liAStep; liShow.
+  liAStep; liShow.
+  liAStep; liShow.
+  liAStep; liShow.
+  liAStep; liShow.
+  liAStep; liShow.
+  liAStep; liShow.
+  liAStep; liShow.
+  liAStep; liShow.
+  liAStep; liShow.
+  liAStep; liShow.
+  liAStep; liShow.
+  liAStep; liShow.
+  liAStep; liShow.
+  liAStep; liShow.
+  liAStep; liShow.
+  liAStep; liShow.
+  liAStep; liShow.
+  liAStep; liShow.
+  liAStep; liShow.
+  liAStep; liShow.
+  liAStep; liShow.
+  liAStep; liShow.
+  liAStep; liShow.
+  liAStep; liShow.
+  liAStep; liShow.
+  liAStep; liShow.
+  liAStep; liShow.
+  liAStep; liShow.
+  liAStep; liShow.
+  liAStep; liShow.
+  liAStep; liShow.
+  liAStep; liShow.
+  liAStep; liShow.
+  liAStep; liShow.
+  liAStep; liShow.
+  liAStep; liShow.
+  liAStep; liShow.
+  liAStep; liShow.
+  liAStep; liShow.
+  liAStep; liShow.
+  liAStep; liShow.
+  liAStep; liShow.
+  liAStep; liShow.
+  liAStep; liShow.
+  liAStep; liShow.
+  liAStep; liShow.
+  liAStep; liShow.
+  liAStep; liShow.
+  liAStep; liShow.
+  liAStep; liShow.
+  liAStep; liShow.
+  liAStep; liShow.
+  liAStep; liShow.
+  liAStep; liShow.
+  liAStep; liShow.
+  liAStep; liShow.
+  liAStep; liShow.
+  liAStep; liShow.
+  liAStep; liShow.
+  liAStep; liShow.
+  liAStep; liShow.
+  liAStep; liShow.
+  liAStep; liShow.
+  liAStep; liShow.
+  liAStep; liShow.
+  liAStep; liShow.
+  liAStep; liShow.
+  liAStep; liShow.
+  liAStep; liShow.
+  liAStep; liShow.
+  liAStep; liShow.
+  liAStep; liShow.
+  liAStep; liShow.
+  liAStep; liShow.
+  liAStep; liShow.
+  liAStep; liShow.
+  liAStep; liShow.
+  liAStep; liShow.
+  liAStep; liShow.
+  liAStep; liShow.
+  liAStep; liShow.
+  liAStep; liShow.
+  liAStep; liShow.
+  liAStep; liShow.
+  liAStep; liShow.
+  liAStep; liShow.
+  liAStep; liShow.
+  liAStep; liShow.
+  liAStep; liShow.
+  liAStep; liShow.
+  liAStep; liShow.
+  liAStep; liShow.
+  liAStep; liShow.
+  liAStep; liShow.
+  liAStep; liShow.
+  liAStep; liShow.
+  liAStep; liShow.
+  liAStep; liShow.
+  liAStep; liShow.
+  liAStep; liShow.
+  liAStep; liShow.
+  liAStep; liShow.
+  liAStep; liShow.
+  liAStep; liShow.
+  liAStep; liShow.
+  liAStep; liShow.
+  liAStep; liShow.
+  liAStep; liShow.
+  liAStep; liShow.
+  liAStep; liShow.
+  liAStep; liShow.
+  liAStep; liShow.
+  liAStep; liShow.
+  liAStep; liShow.
+  liAStep; liShow.
+  liAStep; liShow.
+  liAStep; liShow.
+  liAStep; liShow.
+  liAStep; liShow.
+  liAStep; liShow.
+  liAStep; liShow.
+  liAStep; liShow.
+  liAStep; liShow.
+  liAStep; liShow.
+  liAStep; liShow.
+  liAStep; liShow.
+  liAStep; liShow.
+  liAStep; liShow.
+  liAStep; liShow.
+  liAStep; liShow.
+  liAStep; liShow.
+  liAStep; liShow.
+  liAStep; liShow.
+  liAStep; liShow.
+Abort.
+
 
 (* Lemma test_state2_trace x1 : *)
 (*   (test_state2_global, test_state2_local x1) ~{ seq_module, [Vis (SWriteReg "OUT" [] (Val_Bits [BV{64} 0])) ] }~> -. *)
