theories/automation.v
@@ -76,17 +76,21 @@ Section instances.
       iApply (wp_next_instr_extern with "[$] [$] [$] [$]") => //.
   Qed.
 
-  Lemma li_wp_read_reg r v ann es:
-    (∃ v', r ↦ᵣ v' ∗ (⌜v = v'⌝ -∗ r ↦ᵣ v' -∗ WPasm es)) -∗
-    WPasm (ReadReg r [] v ann :: es).
-  Proof. iDestruct 1 as (?) "[Hr Hwp]". by iApply (wp_read_reg with "Hr"). Qed.
+  Lemma li_wp_read_reg r v ann es al:
+    (∃ v' v'' vread, r ↦ᵣ v' ∗ ⌜read_accessor al v' = Some v''⌝ ∗
+        ⌜read_accessor al v = Some vread⌝ ∗
+       (⌜vread = v''⌝ -∗ r ↦ᵣ v' -∗ WPasm es)) -∗
+    WPasm (ReadReg r al v ann :: es).
+  Proof. iDestruct 1 as (???) "[Hr [% [% Hwp]]]". by iApply (wp_read_reg_acc with "Hr"). Qed.
 
-  Lemma li_wp_write_reg r f v ann es:
-    (∃ v', r ↦ᵣ v' ∗ ⌜f = []⌝ ∗ (r ↦ᵣ v -∗ WPasm es)) -∗
-    WPasm (WriteReg r f v ann :: es).
+  Lemma li_wp_write_reg r al v ann es:
+    (∃ v' v'' vnew, r ↦ᵣ v' ∗
+     ⌜read_accessor al v = Some vnew⌝ ∗ ⌜write_accessor al v' vnew = Some v''⌝ ∗
+     (r ↦ᵣ v'' -∗ WPasm es)) -∗
+    WPasm (WriteReg r al v ann :: es).
   Proof.
-    iDestruct 1 as (?) "[Hr [% Hwp]]"; simplify_eq/=.
-      by iApply (wp_write_reg with "Hr").
+    iDestruct 1 as (???) "[Hr [% [% Hwp]]]"; simplify_eq/=.
+      by iApply (wp_write_reg_acc with "Hr").
   Qed.
 
   Lemma li_wp_branch_address v ann es:
@@ -114,6 +118,21 @@ Section instances.
     WPexp (Manyop op es ann) {{ Φ }}.
   Proof. apply: wpe_manyop. Qed.
 
+  Lemma li_wpe_unop op e Φ ann:
+    WPexp e {{ v1, ∃ v, ⌜eval_unop op v1 = Some v⌝ ∗ Φ v}} -∗
+    WPexp (Unop op e ann) {{ Φ }}.
+  Proof. apply: wpe_unop. Qed.
+
+  Lemma li_wpe_binop op e1 e2 Φ ann:
+    WPexp e1 {{ v1, WPexp e2 {{ v2, ∃ v, ⌜eval_binop op v1 v2 = Some v⌝ ∗ Φ v}} }} -∗
+    WPexp (Binop op e1 e2 ann) {{ Φ }}.
+  Proof. apply: wpe_binop. Qed.
+
+  Lemma li_wpe_ite e1 e2 e3 Φ ann:
+    WPexp e1 {{ v1, WPexp e2 {{ v2, WPexp e3 {{ v3,
+       ∃ b, ⌜v1 = Val_Bool b⌝ ∗ Φ (ite b v2 v3)}} }} }} -∗
+    WPexp (Ite e1 e2 e3 ann) {{ Φ }}.
+  Proof. apply: wpe_ite. Qed.
 End instances.
 
 Ltac liAAsm :=
@@ -123,7 +142,7 @@ Ltac liAAsm :=
     | [] => notypeclasses refine (tac_fast_apply (li_wp_next_instr) _)
     | ?e :: _ =>
       lazymatch e with
-      | ReadReg _ _ _ _ => notypeclasses refine (tac_fast_apply (li_wp_read_reg _ _ _ _) _)
+      | ReadReg _ _ _ _ => notypeclasses refine (tac_fast_apply (li_wp_read_reg _ _ _ _ _) _)
       | WriteReg _ _ _ _ => notypeclasses refine (tac_fast_apply (li_wp_write_reg _ _ _ _ _) _)
       | BranchAddress _ _ => notypeclasses refine (tac_fast_apply (li_wp_branch_address _ _ _) _)
       | Smt (DeclareConst _ (Ty_BitVec _)) _ => notypeclasses refine (tac_fast_apply (li_wp_declare_const_bv _ _ _ _) _)
@@ -142,6 +161,9 @@ Ltac liAExp :=
     lazymatch e with
     | Val _ _ => notypeclasses refine (tac_fast_apply (li_wpe_val _ _ _) _)
     | Manyop _ _ _ => notypeclasses refine (tac_fast_apply (li_wpe_manyop _ _ _ _) _)
+    | Unop _ _ _ => notypeclasses refine (tac_fast_apply (li_wpe_unop _ _ _ _) _)
+    | Binop _ _ _ _ => notypeclasses refine (tac_fast_apply (li_wpe_binop _ _ _ _ _) _)
+    | Ite _ _ _ _ => notypeclasses refine (tac_fast_apply (li_wpe_ite _ _ _ _ _) _)
     | _ => fail "liAExp: unknown exp" e
     end
   end.
